Stuff for proof of substitution, not complete.

Syntax.v
@@ -176,10 +176,10 @@ Inductive is_empty {A} : env A -> Prop :=
 
 Hint Constructors is_empty.
 
-Example is_empty_test : is_empty (None :: None :: @empty ty).
+Example is_empty_ex1 : is_empty (None :: None :: @empty ty).
 Proof. auto. Qed.
 
-Example split_test : exists E,
+Example context_split_ex1 : exists E,
   context_split (insert 0 TyBool empty) (insert 0 TyBool empty) E /\
   is_empty E.
 Proof with auto.
@@ -297,7 +297,7 @@ Proof.
         subst.
         auto.
         auto.
-Qed. (* Automation? *)
+Qed. (* TODO: Automation? *)
 
 Lemma empty_context : forall E E1 E2,
   is_empty E ->
@@ -327,19 +327,6 @@ Proof with auto.
   induction Split...
 Qed.
 
-(* FIXME: delete this probably *)
-Lemma split_misc_lemma : forall E E1 E2 v,
-  context_split (v :: E) E1 E2 ->
-  exists v1 v2 E1' E2', E1 = v1 :: E1' /\ E2 = v2 :: E2' /\ context_split E E1' E2'.
-Proof with auto.
-  intros E E1 E2 v Split.
-  inversion Split as [| ? E1' E2' | ? E1' E2']; subst.
-  Case "left".
-    exists v, None, E1', E2'...
-  Case "right".
-    exists None, v, E1', E2'...
-Qed.
-
 (* In the proof of the lemma below, the proofs for the left and right cases are almost the same.
    The proofs differ only in the first elements of their new amalgamated contexts (E02).
    The first elements for each of the inversion cases are passed as the arguments v1 and v2. *)
@@ -365,34 +352,6 @@ Proof.
   Case "right". split_rotate_crush (None : option ty) v E E0.
 Qed.
 
-(*
-Lemma split_complete_forward : forall E E1 E2 x t,
-  context_split E E1 E2 ->
-  lookup x E = Some t ->
-  (lookup x E1 = Some t) \/ (lookup x E2 = Some t).
-Proof.
-  intros E E1 E2 x t CSplit Lookup.
-  inversion CSplit; subst.
-  destruct H as [sl [Split Len]].
-  induction sl as [ | s sl'].
-  Case "nil - impossible".
-    assert (E = empty).
-      auto using zero_length_empty.
-    subst.
-    exfalso; eauto using lookup_empty_Some.
-  Case "s :: sl'".
-    simpl in Split.
-    destruct E as [ | t0 E'].
-      solve by inversion.
-    simpl in Split.
-    destruct s.
-    SCase "Left".
-      admit.
-    SCase "Right".
-      admit.
-Abort.
-*)
-
 Lemma context_split_length1 : forall E E1 E2,
   context_split E E1 E2 ->
   length E = length E1.
@@ -405,8 +364,7 @@ Lemma context_split_length2 : forall E E1 E2,
   context_split E E1 E2 ->
   length E = length E2.
 Proof.
-  intros E E1 E2 Split.
-  induction Split; simpl; eauto.
+  eauto using context_split_length1, split_commute.
 Qed.
 
 Lemma split_complete_E1 : forall E E1 E2 x t,
@@ -468,6 +426,36 @@ where "L ';' E '|-' t '~:' T" := (has_type L E t T).
 
 Hint Constructors has_type.
 
+(* Predicate for describing whether a variable is contained in a term. *)
+Inductive contains_var : nat -> term -> Prop :=
+  | ContainsVar n : contains_var n (TVar n)
+  | ContainsAbs n e t (CVAbsPre : contains_var (S n) e)
+      : contains_var n (TAbs t e)
+  | ContainsApp1 n e1 e2 (CVApp1Pre : contains_var n e1)
+      : contains_var n (TApp e1 e2)
+  | ContainsApp2 n e1 e2 (CVApp2Pre : contains_var n e2)
+      : contains_var n (TApp e1 e2).
+
+Hint Constructors contains_var.
+
+Example contains_var_ex1 : contains_var 0 (TAbs TyBool (TVar 1)).
+Proof. auto. Qed.
+
+Lemma not_contains_Abs : forall x t e,
+  ~ contains_var x (TAbs t e) ->
+  ~ contains_var (S x) e.
+Proof. auto. Qed.
+
+Lemma not_contains_App1 : forall x e1 e2,
+  ~ contains_var x (TApp e1 e2) ->
+  ~ contains_var x e1.
+Proof. auto. Qed.
+
+Lemma not_contains_App2 : forall x e1 e2,
+  ~ contains_var x (TApp e1 e2) ->
+  ~ contains_var x e2.
+Proof. auto. Qed.
+
 (* Time to prove progress *)
 Theorem progress : forall L E e s t,
   is_empty L ->
@@ -503,11 +491,40 @@ Proof with eauto.
       exists (subst e2 0 e1)...
 Qed.
 
+(* -------------------------- *)
+(* Substitution helper lemmas *)
+(* -------------------------- *)
+
 Lemma insert_none_is_empty : forall {A} (E : env A) E' x,
   is_empty E ->
   raw_insert x None E = E' ->
   is_empty E'.
 Proof. admit. Qed.
+
+Lemma insert_none_is_empty_inversion : forall {A} (E : env A) x,
+  is_empty (raw_insert x None E) -> is_empty E.
+Proof.
+  admit.
+Qed.
+(*
+  intros A E x Empty.
+  generalize dependent E.
+  induction x as [|x']; intros.
+  Case "x = 0".
+    rewrite raw_insert_zero in Empty.
+    inversion Empty. assumption.
+  Case "x = S x'".
+    rewrite raw_insert_successor in Empty.
+    inversion Empty.
+    assert (is_empty (tl E)).
+    auto.
+    assert (E = lookup 0 E :: tl E).
+      admit.
+    rewrite H. auto.
+    Check (hd E).
+    Check lookup_zero.
+    auto.
+*)
 
 Lemma insert_none_split : forall E E1 E2 x,
   context_split E E1 E2 ->
@@ -523,6 +540,44 @@ Proof with eauto.
   Case "x = S x'".
     repeat rewrite raw_insert_successor.
     inversion Split as [|E' E1' E2'|E' E1' E2']...
+Qed.
+
+Lemma split_none_head : forall E E1 E2,
+  context_split (None :: E) E1 E2 ->
+  exists E1' E2', E1 = None :: E1' /\ E2 = None :: E2'.
+Proof.
+  intros E E1 E2 Split.
+  inversion Split; subst; eauto.
+Qed.
+
+(* TODO *)
+Lemma insert_none_split_left : forall E E1 E2 x,
+  context_split (raw_insert x None E) E1 E2 ->
+  (exists E1', E1 = raw_insert x None E1').
+Proof.
+  intros E E1 E2 x Split.
+  generalize dependent E.
+  generalize dependent E1.
+  induction x as [|x']; intros.
+  Case "x = 0".
+    rewrite raw_insert_zero in Split.
+    apply split_none_head in Split. destruct Split as [E1' [E2' [Intro1 Intro2]]].
+    exists E1'.
+    eauto using raw_insert_zero.
+  Case "S x'".
+    rewrite raw_insert_successor in Split.
+    inversion Split; subst.
+    SCase "split_left".
+      subst.
+      admit.
+  admit.
+Qed.
+
+Lemma insert_none_split_right : forall E E1 E2 x,
+  context_split (raw_insert x None E) E1 E2 ->
+  (exists E2', E2 = raw_insert x None E2').
+Proof.
+  eauto using insert_none_split_left, split_commute.
 Qed.
 
 Lemma typing_insert_None : forall L E e t x,
@@ -544,24 +599,129 @@ Proof with (eauto using le_0_n, lt_n_Sm_le, insert_none_is_empty, insert_none_sp
     rewrite insert_insert...
 Qed.
 
-(* If a typing context is used to type an application, then any variable in the context
-   can only be used in either the function OR argument component of the term. *)
-(* WRONG as currently phrased *)
-Lemma app_uniqueness : forall L E e1 e2 v x t tx,
-  lookup x E = Some tx ->
-  L; E |- TApp e1 e2 ~: t ->
-  (subst v x e1 = e1 \/ subst v x e2 = e2).
+(* TODO *)
+Lemma typing_insert_None_reverse : forall L E e t x,
+  L; raw_insert x None E |- e ~: t ->
+  L; E |- unshift x e ~: t.
 Proof.
-  intros L E e1 e2 v x t tx Lookup WT.
-  induction e1; try solve [ left; auto ].
+  intros L E e t x WT.
+  admit.
+Qed.
+
+(* TODO: These two lemmas will be proved with DbLib automation, simpl_unlift_goal. *)
+Lemma unshift_Abs : forall x t e,
+  unshift x (TAbs t e) = TAbs t (unshift (S x) e).
+Proof.
+  admit.
+Qed.
+
+Lemma unshift_App : forall x e1 e2,
+  unshift x (TApp e1 e2) = TApp (unshift x e1) (unshift x e2).
+Proof.
+  admit.
+Qed.
+
+Lemma subst_unshift : forall x e v,
+  ~ contains_var x e ->
+  subst v x e = unshift x e.
+Proof with (eauto using f_equal, not_contains_Abs,
+                        not_contains_App1, not_contains_App2).
+  intros x e v NotContains.
+  generalize dependent x.
+  generalize dependent v.
+  induction e; try solve [simpl_subst_goal; simpl; auto].
   Case "Var".
+    intros.
+    simpl_subst_goal. simpl.
+    destruct (le_gt_dec x n).
+    SCase "x <= n".
+      destruct (le_lt_eq_dec x n)...
+      SSCase "x < n". subst_idx...
+      SSCase "x = n". exfalso. subst...
+    SCase "x > n".
+      subst_idx...
+  Case "Abs".
+    intros.
+    simpl_subst_goal. rewrite unshift_Abs...
+  Case "App".
+    intros.
+    simpl_subst_goal. rewrite unshift_App.
+    rewrite IHe1...
+Qed.
+
+(* TODO: Prove the lemmas like this in DbLib (replace their equivalents) *)
+Lemma raw_insert_eq_insert_1:
+  forall A x a1 a2 (e1 e2 : env A),
+  raw_insert x a1 e1 = raw_insert x a2 e2 ->
+  a1 = a2.
+Proof. admit. Qed.
+
+Lemma raw_insert_eq_insert_3:
+  forall A x1 x2 a1 a2 (e1 e2 : env A),
+  raw_insert x1 a1 e1 = raw_insert x2 a2 e2 ->
+  x1 <> x2 ->
+  exists e y1 y2,
+  e1 = raw_insert y1 a2 e /\
+  e2 = raw_insert y2 a1 e /\
+  shift x1 y1 = x2 /\
+  y2 = (if le_gt_dec x1 y1 then x1 else x1 - 1).
+Proof.
+  admit.
+Qed.
+
+Lemma typing_without_var : forall L E e x t,
+  L; raw_insert x None E |- e ~: t -> ~ contains_var x e.
+Proof with (eauto using raw_insert_eq_insert_1, le_0_n).
+  unfold not.
+  intros L E e x t WT Contains.
+  generalize dependent E.
+  generalize dependent x.
+  generalize dependent t.
+  induction e; try solve [intros; solve by inversion].
+  Case "Var".
+    intros.
     destruct (eq_nat_dec x n).
-    SCase "x = n". admit.
+    SCase "x = n".
+      subst x.
+      inversion WT; subst.
+      assert (Some t = None)...
+      solve by inversion.
     SCase "x <> n".
-      left.
-      simpl_subst_goal.
-      (* Problematic because vars change their internal index. *)
-Abort.
+      inversion Contains...
+  Case "TAbs".
+    intros.
+    inversion WT; subst.
+    rewrite insert_insert in AbsPre...
+    inversion Contains; subst...
+  Case "TApp".
+    intros.
+    inversion Contains.
+    (* TODO: deduplicate *)
+    SCase "e1 contains x".
+      subst.
+      inversion WT. subst.
+      apply insert_none_split_left in AppPreSplit.
+      destruct AppPreSplit as [E1' IntroE1'].
+      subst...
+    SCase "e2 contains x".
+      subst.
+      inversion WT. subst.
+      apply insert_none_split_right in AppPreSplit.
+      destruct AppPreSplit as [E1' IntroE1'].
+      subst...
+Qed.
+
+Lemma typing_insert_none_subst : forall L E e x junk t,
+  L; raw_insert x None E |- e ~: t ->
+  L; E |- subst junk x e ~: t.
+Proof.
+  intros L E e x junk t WT.
+  remember WT as H eqn:Junk; clear Junk.
+  apply typing_without_var in H.
+  apply subst_unshift with (v := junk) in H.
+  rewrite H.
+  eauto using typing_insert_None_reverse.
+Qed.
 
 Lemma substitution: forall L E2 e2 t1 t2 x,
   L; insert x t1 E2 |- e2 ~: t2 ->
@@ -572,7 +732,7 @@ Proof with (eauto using typing_insert_None).
   intros L E2 e2 t1 t2 x WT2 E E1 e1 WT1 Split.
   dependent induction WT2; simpl_subst_goal; try solve [exfalso; eauto using insert_empty_contra].
   Case "Var".
-    (* FIXME: naming of x is weird here *)
+    (* XXX: naming of x is weird here *)
     apply insert_empty_inversion in x...
     destruct x as [XEq [TEq E2Eq]].
     subst.
@@ -601,28 +761,34 @@ Proof with (eauto using typing_insert_None).
       admit.
     apply HasTyApp with (E1 := E1) (E2 := E02) (t1 := t0).
       assumption.
-    admit. (* Need something here about raw_insert and subst and shift *)
+    subst E1'; eauto using typing_insert_none_subst.
     apply IHWT2_2 with (E1 := E0) (E2 := E2) (t1 := t1).
       rewrite E2Intro; auto. (* messy *)
       assumption.
       assumption.
 Qed.
 
-(* Preservation *)
-Theorem preservation : forall e e' s s' t,
-  empty; empty |- e ~: t ->
+(* Preservation - TODO *)
+Theorem preservation : forall L E e e' s s' t,
+  is_empty L ->
+  is_empty E ->
+  L; E |- e ~: t ->
   step s e s' e' ->
-  empty; empty |- e' ~: t.
+  L; E |- e' ~: t.
 Proof with eauto.
-  intros e e' s s' t WT ST.
+  intros L E e e' s s' t EmptyL EmptyE WT ST.
   generalize dependent t.
   induction ST.
   Case "Beta reduction".
     intros.
     inversion WT; subst.
-    apply empty_context in H3. destruct H3. subst. (* TACME *)
-    inversion H6; subst.
-    eauto using substitution.
+    apply empty_context in AppPreSplit. destruct AppPreSplit. subst.
+    inversion AppPreWT1; subst.
+    apply substitution with (E1 := E2) (t1 := t1) (E2 := E1).
+      assumption.
+      assumption.
+      admit. (* need a thing about empty context splits *)
+      assumption.
   Case "App1 stepping".
     intros.
     inversion WT.
